discovered correct invariants variations using expect

leetcode/preorderTraversal.dfy
@@ -2,6 +2,7 @@ include "./invertTree.dfy"
 
 module PreorderTraversal {
     import opened InvertBinaryTree
+    import Std.Collections.Seq
     method SetToSeq<T>(s: set<T>) returns (xs: seq<T>)
       ensures multiset(s) == multiset(xs)
     {
@@ -16,19 +17,73 @@ module PreorderTraversal {
       }
     }
 
+    function toSet<T>(s: seq<T>): set<T> 
+      decreases |s|
+    {
+      if s == [] then {} else toSet(s[..|s|-1])+{s[|s|-1]}
+    }
+
     function children(node: TreeNode): set<TreeNode> 
-        reads node, node.repr
+        // requires node.Valid()
+        reads node
+        // ensures children(node) < node.repr
+        // ensures node !in children(node)
     {
         (if node.right != null then {node.right} else {}) + 
         (if node.left != null then {node.left} else {})
     }
     function childStack(node: TreeNode?): seq<TreeNode> 
-        reads node
+        reads if node == null then {} else node.repr
+        requires node != null ==> node.Valid()
+        ensures forall x :: x in childStack(node) ==> x.Valid()
     {
         if node == null then [] else
-        (if node.right != null then [node.right] else []) + 
-        (if node.left != null then [node.left] else [])
+        (if node.right != null then 
+        assert node.Valid();
+        assert node.right.Valid();
+        [node.right] else []) + 
+        (if node.left != null then
+        assert node.Valid();
+        assert node.left.Valid();
+         [node.left] else [])
     }
+
+    function rightStack(node: TreeNode): seq<TreeNode> 
+        reads node
+        // requires node.Valid()
+    {
+      if node.right != null then [node.right] else []
+    }
+
+    function rightStackVisited(node: TreeNode, visited: set<TreeNode>): seq<TreeNode> 
+        reads node
+        // requires node.Valid()
+    {
+      if node.right != null && node.right !in visited then [node.right] else []
+    }
+
+    lemma childStackLemma(node: TreeNode?)
+        requires node != null ==> node.Valid()
+        ensures node == null ==> childStack(node) == []
+        ensures node != null && node.left == null && node.right == null ==> childStack(node) == []
+        ensures node != null && node.left != null && node.right == null ==> childStack(node) == [node.left]
+        ensures node != null && node.left == null && node.right != null ==> childStack(node) == [node.right]
+        ensures node != null && node.left != null && node.right != null ==> childStack(node) == [node.right, node.left]
+        ensures node != null ==> TreeUnion(childStack(node)) == node.repr-{node}
+      {
+        if node == null {
+
+        } else{
+          if node.right != null && node.left != null {
+              assert node.right.repr + node.left.repr == node.repr - {node};
+              TreeUnionConcat([node.right],[ node.left]);
+              assert TreeUnion(childStack(node)) == node.right.repr + node.left.repr;
+            } else if node.right != null && node.left == null {
+            } else if node.right == null && node.left != null {
+            }else {
+            }
+        }
+      }
 
     function mapNodes(ss: seq<TreeNode>): seq<int> 
         reads set i | 0 <= i < |ss| :: ss[i]
@@ -36,10 +91,83 @@ module PreorderTraversal {
         if ss == [] then [] else [ss[0].val]+mapNodes(ss[1..])
     }    
 
+    function parentStack(node: TreeNode): seq<TreeNode> 
+      reads node, node.repr
+      requires node.Valid()
+    {
+      if |childStack(node)| > 0 then [node] else []
+    }
+
+    lemma parentStackLemma(node: TreeNode)
+      requires node.Valid()
+      ensures forall x :: x in parentStack(node) ==> x.Valid()
+    {
+
+    }
+
+    // ghost function AllReprs(ss: seq<TreeNode>): set<TreeNode>
+    //   reads ss, ss[0]
+    // {
+    //   if ss == []  then {} else ss[0].repr + AllReprs(ss[1..])
+    // }
+
+    function setUnion<T>(xs: seq<set<T>>): set<T> {
+      if xs == [] then {} else xs[0] + setUnion(xs[1..])
+    }
+
+    function reprUnion(xs: seq<TreeNode>): set<TreeNode> 
+      reads xs
+      ensures forall x :: x in xs ==> x.repr <= reprUnion(xs)
+    {
+      if xs == [] then {} else xs[0].repr + reprUnion(xs[1..])
+    }
+
+    function pruneParents(ss: seq<TreeNode>, visited: set<TreeNode>): seq<TreeNode> 
+      // reads (set i | 0 <= i < |ss| :: ss[i]) + setUnion(Seq.Map((x: TreeNode) reads x => x.repr, ss))
+      reads (set i | 0 <= i < |ss| :: ss[i])
+        // reads AllReprs(ss)
+        // reads ss
+        // requires forall x :: x in ss ==> x.Valid()
+        ensures forall x :: x in pruneParents(ss, visited) ==> x in ss
+    {
+      if ss != [] then if children(ss[|ss|-1]) <= visited then pruneParents(ss[..|ss|-1], visited) else ss else []
+    }
+
+    lemma pruneParentsLemma(ss: seq<TreeNode>, visited: set<TreeNode>)
+      requires AllAncestors(ss)
+      ensures AllAncestors(pruneParents(ss, visited))
+    {
+
+    }
+
   predicate compare(a: TreeNode, b: TreeNode)
     reads a, b
   {
     a.val <= b.val
+  }
+
+  predicate AllAncestors(ts: seq<TreeNode>) 
+      reads set i | 0 <= i < |ts| :: ts[i]
+  {
+    forall i :: 0 <= i < |ts|-1 ==> childOf(ts[i+1], ts[i])
+  }
+
+  predicate AllAncestorsDesc(ts: seq<TreeNode>) 
+      reads set i | 0 <= i < |ts| :: ts[i], reprUnion(ts), set i | 0 <= i < |ts| :: ts[i].left, set i | 0 <= i < |ts| :: ts[i].right
+  {
+    forall i :: 0 <= i < |ts|-1 ==> childOf(ts[i+1], ts[i]) || descOf(ts[i+1], ts[i])
+  }
+
+  predicate childOf(a: TreeNode, b: TreeNode)
+    reads a,b
+  {
+    a == b.left || a == b.right
+  }
+
+  predicate descOf(a: TreeNode, b: TreeNode)
+    reads a,b,b.repr, if b.left != null then {b.left} else {}, if b.right != null then {b.right} else {}
+  {
+    (b.left != null && a in b.left.repr) || (b.right != null && a in b.right.repr)
   }
 
 lemma ThereIsAMinimum(s: set<TreeNode>)
@@ -115,74 +243,299 @@ lemma ThereIsAMinimum(s: set<TreeNode>)
       forall x,y :: x in ss && y in ss && x != y ==> x.val != y.val 
     }
 
+    ghost predicate AllDisjoint(ts: seq<TreeNode>)
+        reads set x | 0 <= x < |ts| :: ts[x]
+    {
+        forall x, y :: 0 <= x < y < |ts| && x != y ==> ts[x].repr !! ts[y].repr
+    }
 
-    // function mapNodeSet(ss: set<TreeNode>): set<int> 
-    //   reads ss
-    //   requires uniqueNodes(ss)
-    // {
-    //     if ss == {} then 
-    //         {}
-    //     else 
-    //       ThereIsAMinimum(ss);
-    //       // ThereIsAMinimumG(ss);
-    //       var s :| s in ss && forall ys :: ys in ss ==> compare(s, ys);
-    //       {s.val}+mapNodeSet(ss - {s})
-    // }    
+    lemma  AllDisjointMaint(stack: seq<TreeNode>, current: TreeNode)
+        requires |stack| > 0
+        requires AllDisjoint(stack)
+        requires forall x :: x in stack ==> x.Valid()
+        requires current == stack[|stack|-1]
+        ensures current.left != null && current.right != null ==> AllDisjoint(stack[..|stack|-1]+[current.right, current.left])
+        ensures current.left != null && current.right == null ==> AllDisjoint(stack[..|stack|-1]+[current.left])
+        ensures current.left == null && current.right != null ==> AllDisjoint(stack[..|stack|-1]+[current.right])
+        ensures current.left == null && current.right == null ==> AllDisjoint(stack[..|stack|-1])
+    {
+            assert current.Valid();
+            if current.right != null && current.left != null {
+                // assert AllDisjoint(stack[..|stack|-1]+[current.right, current.left]);
+            } else if current.right != null && current.left == null {
+                assert current.right.repr < current.repr;
+                // assert AllDisjoint(stack[..|stack|-1]+[current.right]);
+            } else if current.right == null && current.left != null {
+                // assert AllDisjoint(stack[..|stack|-1]+[current.left]);
+            }else {
+                // assert AllDisjoint(stack[..|stack|-1]);
+            }
+    }
+
+    lemma  TreeUnionMaint(stack: seq<TreeNode>, current: TreeNode, unvisited: set<TreeNode>)
+        requires |stack| > 0
+        requires unvisited == TreeUnion(stack)
+        requires AllDisjoint(stack)
+        requires forall x :: x in stack ==> x.Valid()
+        requires current == stack[|stack|-1]
+        ensures TreeUnion(stack[..|stack|-1]+childStack(current)) == unvisited-{current}
+    {
+        childStackLemma(current);
+        // assert current.Valid();
+        assert stack == stack[..|stack|-1]+[stack[|stack|-1]];
+        TreeUnionConcat(stack[..|stack|-1],[stack[|stack|-1]]);
+        // assert TreeUnion(stack) == TreeUnion(stack[..|stack|-1])+TreeUnion([stack[|stack|-1]]);
+        assert TreeUnion([stack[|stack|-1]]) == current.repr;
+        assert TreeUnion(stack[..|stack|-1]) !! current.repr by {
+            forall x | x in TreeUnion(stack[..|stack|-1])
+                ensures x !in current.repr
+            {
+                // var xx :| xx in stack[..|stack|-1] && x in xx.repr;
+                TreeUnionLemma(stack[..|stack|-1]);
+                var k :| 0 <= k < |stack[..|stack|-1]| && x in stack[..|stack|-1][k].repr;
+                assert stack[..|stack|-1][k].repr !! current.repr;
+            }
+        }
+        // assert TreeUnion(stack[..|stack|-1]) == unvisited-current.repr;
+        if current.left != null && current.right != null {
+            assert current.right.repr + current.left.repr + {current} == current.repr;
+            assert current.right.repr + current.left.repr == current.repr - {current};
+            TreeUnionConcat([current.right],[current.left]);
+            // assert TreeUnion([current.right, current.left]) == current.right.repr + current.left.repr;
+            TreeUnionConcat(stack[..|stack|-1], [current.right, current.left]);
+        } else if current.left != null && current.right == null {
+            assert current.left.repr == current.repr - {current};
+            TreeUnionConcat(stack[..|stack|-1], [current.left]);
+            
+        }else if current.left == null && current.right != null {
+            assert current.right.repr == current.repr - {current};
+            TreeUnionConcat(stack[..|stack|-1], [current.right]);
+
+        }else if current.left == null && current.right == null {
+            TreeUnionConcat(stack[..|stack|-1], []);
+
+        }
+    }
+
+    lemma {:verify false} {:vcs_split_on_every_assert} traverseMaint(
+        root: TreeNode,
+        result: seq<TreeNode>,
+        visited: set<TreeNode>,
+        stack: seq<TreeNode>,
+        parents: seq<TreeNode>,
+        unvisited: set<TreeNode>,
+        i: int)
+      requires |stack| > 0 
+      requires root.Valid()
+      requires toSet(result) == visited
+      requires forall x :: x in parents ==> x.Valid()
+      requires forall x :: x in stack ==> x.Valid()
+      requires forall x :: x in stack ==> x in root.repr
+      requires forall x :: x in visited ==> x in root.repr
+      requires AllAncestors(parents)
+      requires stack == [root] ==> parents == []
+      requires parents != [] ==> childOf(stack[ |stack| -1], parents[ |parents| -1])
+      requires parents != [] ==> stackPred2(stack, parents, visited)
+      requires unvisited !! visited
+      requires unvisited + visited == root.repr
+      // requires visited <= root.repr
+      // requires |visited| <= |root.repr|
+      requires forall x :: x in stack ==> x in unvisited
+      requires AllDisjoint(stack)
+      requires unvisited == TreeUnion(stack)
+      // requires i == |result|
+      // requires i == |visited|
+      // requires 0 <= i <= |PreorderTraversal(root)|
+      // requires result == PreorderTraversal(root)[..i]
+      // requires |stack| > 0 && i < |PreorderTraversal(root)| ==> stack[|stack|-1] == PreorderTraversal(root)[i]
+      ensures AllAncestors(pruneParents(parents+parentStack(stack[|stack|-1]), visited+{stack[|stack|-1]}))
+      ensures forall x :: x in pruneParents(parents+parentStack(stack[|stack|-1]), visited+{stack[|stack|-1]}) ==> x.Valid()
+      // ensures stack[..|stack|-1]+childStack(stack[|stack|-1]) == 
+    {
+      assert forall x :: x in parents+parentStack(stack[|stack|-1]) ==> x.Valid() by {
+        forall x | x in parents+parentStack(stack[|stack|-1])
+          ensures x.Valid()
+        {
+          if x in parents {
+            assert x.Valid();
+          }else{
+          parentStackLemma(stack[|stack|-1]);
+            assert x in parentStack(stack[|stack|-1]);
+            assert x.Valid();
+          }
+        }
+      }
+      assert forall x :: x in pruneParents(parents+parentStack(stack[|stack|-1]), visited+{stack[|stack|-1]}) ==> x.Valid() by {
+        forall x | x in pruneParents(parents+parentStack(stack[|stack|-1]), visited+{stack[|stack|-1]})
+          ensures x.Valid()
+        {
+          assert x in parents+parentStack(stack[ |stack|-1]);
+          assert x.Valid();
+        }
+      }
+      assert AllAncestors(pruneParents(parents+parentStack(stack[|stack|-1]), visited+{stack[|stack|-1]})) by {
+        assert AllAncestors(parents+parentStack(stack[|stack|-1]));
+        pruneParentsLemma(parents+parentStack(stack[|stack|-1]), visited+{stack[|stack|-1]});
+      }
+      var newParents := pruneParents(parents, visited+{stack[|stack|-1]})+parentStack(stack[|stack|-1]);
+      var newStack := stack[..|stack|-1]+childStack(stack[|stack|-1]);
+      if newParents != [] && parents != [] {
+        if |childStack(stack[|stack|-1])| > 0 {
+          assert parentStack(stack[|stack|-1]) == [stack[|stack|-1]];
+        }else{
+          assert parentStack(stack[|stack|-1]) == [];
+        }
+        // assert childOf(newStack[|newStack|-1], newParents[|newParents|-1]);
+        assert stackPred2(newStack, newParents, visited+{stack[|stack|-1]}) by {
+          if stack == Seq.Flatten(Seq.Map(rightStack, parents)) {
+
+          }else if stack == Seq.Flatten(Seq.Map(rightStack, parents[..|parents|-1]))+childStack(parents[|parents|-1]) {
+
+          }
+        }
+      }
+    }
+
+    predicate stackPred(stack: seq<TreeNode>, parents: seq<TreeNode>) 
+      reads parents, set i | 0 <= i < |parents| :: parents[i], reprUnion(parents)
+      requires forall parent :: parent in parents ==> parent.Valid()
+    {
+      stack == Seq.Flatten(Seq.Map(rightStack, parents)) || (|parents| > 0 && stack == Seq.Flatten(Seq.Map(rightStack, parents[..|parents|-1]))+childStack(parents[|parents|-1]))
+    }
+
+    predicate stackPred2(stack: seq<TreeNode>, parents: seq<TreeNode>, visited: set<TreeNode>) 
+      reads parents, set i | 0 <= i < |parents| :: parents[i], reprUnion(parents)
+      requires forall parent :: parent in parents ==> parent.Valid()
+    {
+      var visitMap := (x: TreeNode) reads x => rightStackVisited(x, visited);
+      stack == Seq.Flatten(Seq.Map(visitMap, parents)) || (|parents| > 0 && stack == Seq.Flatten(Seq.Map(visitMap, parents[..|parents|-1]))+childStack(parents[|parents|-1]))
+    }
     
-    method Traverse(root: TreeNode) returns (result: seq<TreeNode>)
+    method {:verify false} {:vcs_split_on_every_assert} Traverse(root: TreeNode) returns (result: seq<TreeNode>)
         requires root.Valid()
-        decreases *
+        ensures result == PreorderTraversal(root)
     {
         var stack := [root];
+        var pro := PreorderTraversal(root);
+        assert |pro| == root.TreeSize();
         var i := 0;
         result := [];
         var visited: set<TreeNode> := {};
-        var visiteds: seq<TreeNode> := [];
         var unvisited: set<TreeNode> := root.repr;
+        assert |unvisited| == |root.repr|;
         var parents: seq<TreeNode> := [];
         var parentIndices: seq<int> := [];
         while |stack| > 0 
+            invariant toSet(result) == visited
             invariant |parents| == |parentIndices|
-            decreases *
+            invariant forall x :: x in parents ==> x.Valid()
+            invariant forall x :: x in stack ==> x.Valid()
+            invariant forall x :: x in stack ==> x in root.repr
+            invariant forall x :: x in visited ==> x in root.repr
+            invariant unvisited !! visited
+            invariant unvisited + visited == root.repr
+            invariant visited <= root.repr
+            invariant |visited| <= |root.repr|
+
+            invariant forall x :: x in stack ==> x in unvisited
+            invariant AllDisjoint(stack)
+            invariant unvisited == TreeUnion(stack)
+            invariant i == |result|
+            invariant i == |visited|
+            invariant 0 <= i <= |pro|
+            invariant result == pro[..i]
+            invariant |stack| > 0 && i < |pro| ==> stack[|stack|-1] == pro[i]
+            decreases |root.repr| - i
         {
             print "i: ", i, "\n";
             print "pre ", "result ", mapNodes(result), " \n";
             print "pre ", "stack ", mapNodes(stack), " \n";
             print "pre ", "parents ", mapNodes(parents), " \n";
             print "pre ", "parentIndices ", parentIndices, " \n";
-            print "pre ", "visited ", mapNodes(visiteds), " \n";
             var current := stack[|stack|-1];
+            expect parents != [] ==> stackPred2(stack, parents, visited), "Before stack pred is true";
+            print "pre ", "current ", current.val, "\n";
             var stack' := childStack(current);
             if |stack'| > 0 {
                 parentIndices := parentIndices + [i];
-                parents := parents + [current];
+                parents := parents + parentStack(current);
+            }
+            expect AllAncestors(parents), "Before stack AllAncestors true";
+            assert children(current) <= current.repr;
+            TreeUnionMaint(stack, current, unvisited);
+            AllDisjointMaint(stack, current);
+
+            ChildNodesAreValid(root, current);
+            assert stack == stack[..|stack|-1]+[stack[|stack|-1]];
+            assert forall x :: x in stack[..|stack|-1]+stack' ==> x.Valid() by {
+              forall x | x in stack[..|stack|-1]+stack'
+                ensures x.Valid()
+              {
+                if x in stack[..|stack|-1] {
+                  assert x in stack;
+                }else{
+                  assert x in stack';
+                }
+              }
+            }
+            assert forall x :: x in stack[..|stack|-1]+stack' ==> x in unvisited-{current} by {
+              forall x | x in stack[..|stack|-1]+stack'
+                ensures x in unvisited-{current}
+              {
+                if x in stack[..|stack|-1] {
+                  assert x in stack;
+                  assert x != current;
+                  assert x in unvisited-{current};
+                }else{
+                  TreeUnionConcat(stack[..|stack|-1],[stack[|stack|-1]]);
+                  assert TreeUnion([stack[|stack|-1]]) == current.repr;
+                  assert children(current) < current.repr;
+                  assert x in children(current);
+                  assert x != current;
+                  childStackLemma(current);
+                  TreeUnionConcat(stack[..|stack|-1],stack');
+                  assert TreeUnion(stack') == current.repr-{current};
+                  assert x in unvisited-{current};
+                }
+              }
             }
             stack := stack[..|stack|-1]+stack';
             result := result + [current];
             visited := visited + {current};
-            visiteds := visiteds + [current];
             unvisited := unvisited-{current};
-            if |parents| > 0 { 
-              var childnodes := SetToSeq(children(parents[|parents|-1]));
-              print "children, ", mapNodes(childnodes);
-            }
-            if |parents| > 0 && children(parents[|parents|-1]) <= visited {
-                parents := parents[..|parents|-1];
-                parentIndices := parentIndices[..|parentIndices|-1];
-            }
+            // if |parents| > 0 { 
+            //   var childnodes := SetToSeq(children(parents[|parents|-1]));
+            //   print "children, ", mapNodes(childnodes);
+            // }
+            parents := pruneParents(parents, visited);
+          
+            // if (|parents| > 0) && (children(parents[|parents|-1]) <= visited)
+            // {
+            //     parents := parents[..|parents|-1];
+            //     // parentIndices := parentIndices[..|parentIndices|-1];
+            // }
+
+            // if (|parents| > 0) && (children(parents[|parents|-1]) <= visited)
+            // {
+            //     parents := parents[..|parents|-1];
+            //     // parentIndices := parentIndices[..|parentIndices|-1];
+            // }
+            assume {:axiom} forall p :: p in parents ==> p.Valid();
+         
 
             print "post ", "result ", mapNodes(result), " \n";
             print "post ", "stack ", mapNodes(stack), " \n";
             print "post ", "parents ", mapNodes(parents), " \n";
             print "post ", "parentIndices ", parentIndices, " \n";
-            print "post ", "visited ", mapNodes(visiteds), " \n";
+            expect parents != [] ==> stackPred2(stack, parents, visited), "After pred works";
+            expect AllAncestors(parents), "after stack AllAncestors true";
             i := i + 1;
         }
+        assert result == PreorderTraversal(root)[0..|PreorderTraversal(root)|];
         return result;
     }
 
     method Main() 
-      decreases *
     {
         var u := new TreeNode(20, null, null);
         var v := new TreeNode(21, null, null);
